\documentclass[10pt]{article}
\usepackage[usenames]{color} %used for font color
\usepackage{amssymb} %maths
\usepackage{amsmath} %maths
\usepackage[utf8]{inputenc} %useful to type directly diacritic characters
\begin{document}
\begin{align*}f(x) &= f_0 + f_1x + f_2x^2 + ... \\
g(x) &= g_0 + g_1x + g_2x^2 + ... \\
h(x) &= f(x)g(x) = \underbrace{f_0g_0}_{h_0} + \underbrace{(f_0g_1+f_1g_0)}_{h_1}x + \underbrace{(f_0g_2 + f_1g_1 + f_2g_0)}_{h_2}x^2 + ..., \\
h_k &= \sum_{m=0}^k  f_m g_{k-m}. \\
h(x) &= g(f(x)) = \underbrace{g(f_0)}_{h_0} + \underbrace{g'f_1}_{h_1}x + \underbrace{(0.5 g''f_1 f_1 + g'f_2)}_{h_2}x^2 + ... \\
\mathbf{B}_k &=- \mathbf{A}_0^{-1}\sum_{m=1}^{k} \mathbf{A}_{m} \cdot \mathbf{B}_{k-m}. \\
\frac{df}{dz} &= \frac{d}{dt}f(x_1+tc_1,x_2+tc_2,x_3+tc_3)\Big|_{t=0} = c_1 \frac{\partial f}{\partial x_1} + c_2 \frac{\partial f}{\partial x_2} + c_2 \frac{\partial f}{\partial x_2}, \\
\frac{d^2f}{dz^2} &=\frac{d^2}{dt^2}f(x_1+tc_1,x_2+tc_2,x_3+tc_3)\Big|_{t=0} = \sum_{i,j=1..3} c_i c_j \frac{\partial^2f}{\partial x_i\partial x_j}, \\
\frac{df}{dt}\Big|_{\mathbf{c}=(1,0,0)} &= \frac{\partial f}{\partial x_1},~~~~~
\frac{df}{dt}\Big|_{\mathbf{c}=(0,1,0)} = \frac{\partial f}{\partial x_2},~~~~~
\frac{df}{dt}\Big|_{\mathbf{c}=(0,0,1)} = \frac{\partial f}{\partial x_3}, \\
\frac{d^2f}{dt^2}\Big|_{\mathbf{c}=(1,0,0)} &= \frac{\partial^2 f}{\partial x_1^2},~~~~~
\frac{d^2f}{dt^2}\Big|_{\mathbf{c}=(0,1,0)} = \frac{\partial^2 f}{\partial x_2^2},~~~~~
\frac{d^2f}{dt^2}\Big|_{\mathbf{c}=(0,0,1)} = \frac{\partial^2 f}{\partial x_3^2}, \\
\frac{d^2f}{dt^2}\Big|_{\mathbf{c}=(1,1,0)} &= \frac{\partial^2 f}{\partial x_1^2}+\frac{\partial^2 f}{\partial x_2^2}+2\frac{\partial^2 f}{\partial x_1x_2}, \\
\frac{d^2f}{dt^2}\Big|_{\mathbf{c}=(1,0,1)} &= \frac{\partial^2 f}{\partial x_1^2}+\frac{\partial^2 f}{\partial x_3^2}+2\frac{\partial^2 f}{\partial x_1x_3}, \\
\frac{d^2f}{dt^2}\Big|_{\mathbf{c}=(0,1,1)} &= \frac{\partial^2 f}{\partial x_2^2}+\frac{\partial^2 f}{\partial x_3^2}+2\frac{\partial^2 f}{\partial x_2x_3}. \\
\frac{\partial^2 f}{\partial x_1x_2} &= \frac{1}{2}\left(\frac{d^2f}{dt^2}\Big|_{\mathbf{c}=(1,1,0)} - \frac{\partial^2 f}{\partial x_1^2}-\frac{\partial^2 f}{\partial x_2^2}\right). \\
\frac{\partial^{|\mathbf{i}|} f}{\partial x_1^{i_1}\partial x_2^{i_2}...\partial x_n^{i_n}} &= \sum_{|\mathbf{c}|=d}\frac{\partial^d f}{\partial t^d}\Big|_{\mathbf{c}}\cdot g_{\mathbf{i},\mathbf{c}}, \\
g_{\mathbf{i},\mathbf{c}} &= \sum_{0<\mathbf{k}\leq\mathbf{i}}(-1)^{|\mathbf{i}-\mathbf{k}|}{\mathbf{i}\choose\mathbf{k}}{d\mathbf{k}/|\mathbf{k}|\choose\mathbf{c}}\left(|\mathbf{k}|/d\right)^{|\mathbf{i}|}.
\end{align*}
\end{document}